level based API

theories/shared_ref.v
@@ -3,24 +3,24 @@ From iris.base_logic.lib Require Export own na_invariants invariants iprop.
 From iris.heap_lang Require Import lang proofmode notation.
 From iris.algebra Require Import agree.
 
-Section shared_ref.
+Section concurrent_stable_ref.
 
 Context `{!heapGS Σ}.
 
 Let N := nroot .@ "sref".
 
-Definition sref (ℓ : loc) (π : val -> iProp Σ) : iProp Σ :=
-  inv N (∃ v, π v ∗ ℓ ↦ v).
+Definition csref (ℓ : loc) (ϕ : val -> iProp Σ) : iProp Σ :=
+  inv N (∃ v, ϕ v ∗ ℓ ↦ v).
 
-Notation "l ⤇ π" := (sref l π) (at level 60).
+Notation "l ⤇ ϕ" := (csref l ϕ) (at level 60).
 
-Theorem pers_sref : forall ℓ π, Persistent (sref ℓ π).
+Theorem pers_sref : forall ℓ ϕ, Persistent (csref ℓ ϕ).
 Proof. apply _. Qed.
 
-Variable π : val -> iProp Σ.
+Variable ϕ : val -> iProp Σ.
 
-Theorem sref_alloc (v : val) :
-  {{{ π v }}} ref v {{{ ℓ, RET #ℓ; ℓ ⤇ π }}}.
+Theorem csref_alloc (v : val) :
+  {{{ ϕ v }}} ref v {{{ ℓ, RET #ℓ; ℓ ⤇ ϕ }}}.
 Proof.
   iIntros (ψ) "Hv Hψ".
   wp_alloc ℓ as "Hℓ".
@@ -30,8 +30,8 @@ Proof.
   iExists v. by iFrame.
 Qed.
 
-Theorem sref_load `{forall x, Persistent (π x)} (ℓ : loc) :
-  {{{ ℓ ⤇ π }}} ! #ℓ {{{ v', RET v'; π v' }}}.
+Theorem csref_load `{forall x, Persistent (ϕ x)} (ℓ : loc) :
+  {{{ ℓ ⤇ ϕ }}} ! #ℓ {{{ v', RET v'; ϕ v' }}}.
 Proof.
   iIntros (ψ) "#ι Hψ".
   iInv "ι" as "(%v' & #Hv' & Hℓ)".
@@ -41,8 +41,8 @@ Proof.
   - by iApply "Hψ".
 Qed.
 
-Theorem sref_store (ℓ : loc) (x : val) :
-  {{{ ℓ ⤇ π ∗ π x }}} #ℓ <- x {{{ RET #(); True }}}.
+Theorem csref_store (ℓ : loc) (x : val) :
+  {{{ ℓ ⤇ ϕ ∗ ϕ x }}} #ℓ <- x {{{ RET #(); True }}}.
 Proof.
   iIntros (ψ) "(#ι & Hx) Hψ".
   iInv "ι" as "(%v' & Hv' & Hℓ)".
@@ -52,106 +52,190 @@ Proof.
   iExists x. by iFrame.
 Qed.
 
-End shared_ref.
+End concurrent_stable_ref.
 
-Section alloc.
-  Context `{!heapGS Σ} `{!na_invG Σ}.
-  Theorem na_pool_alloc :
-    ⊢ |==> ∃ p : gname, na_own p ⊤.
-  Proof. by apply na_alloc. Qed.
-End alloc.
+Section namespacing.
+  (* This section describes the namespaces used by the na_invariants *)
+  Context `{!na_invG Σ}.
+
+  (* The main namespace used by cadeques *)
+  Definition NKot := nroot .@ "stable ref".
+
+  (* Ξ n is the namespace of cadeques at depth n or deeper *)
+  Fixpoint Ξ (n : nat) : namespace :=
+    match n with
+    | 0 => NKot
+    | S n => Ξ n .@ (S n)
+    end.
+
+  Lemma next_stage : forall n, ↑Ξ (S n) ⊆@{coPset} ↑Ξ n.
+  Proof.
+    move=> n.
+    by apply nclose_subseteq.
+  Qed.
+
+  (* W n is the right to write in a cadeque of depth exactly n *)
+  Definition W n := Ξ n .@ 0.
+
+  Lemma incl_trans : forall A B C : coPset, A ⊆ B -> B ⊆ C -> A ⊆ C.
+  Proof.
+    move=> A B C H K i L.
+    by apply H, K in L.
+  Qed.
+
+  (* Accessing stage n cadeques allows for writing in them *)
+  Lemma access_stage : forall n, ↑W n ⊆@{coPset} ↑Ξ n.
+  Proof.
+    move=> n.
+    apply nclose_subseteq.
+  Qed.
+
+  Lemma next_stage_split : forall n, ↑Ξ (S n) ⊆@{coPset} difference (↑Ξ n) (↑W n).
+  Proof.
+    move=> n.
+    apply namespaces.coPset_subseteq_difference_r.
+    - rewrite /W /=. by apply ndot_ne_disjoint.
+    - apply next_stage.
+  Qed.
+
+  (* Access to depth n is writing at level n & access to depth (n+1) & a rest σ *)
+  Property own_next_stage : forall ρ n, ∃ σ, na_own ρ (difference (↑Ξ n) (↑W n)) ∗-∗ (na_own ρ (↑Ξ (S n)) ∗ na_own ρ σ).
+  Proof.
+    move=> ρ n.
+    set (H := next_stage_split n).
+    apply subseteq_disjoint_union_L in H as [σ [Heq Hdisj]].
+    exists σ. iSplitL.
+    - iIntros "H".
+      rewrite Heq.
+      by iApply na_own_union.
+    - iIntros "[H K]".
+      rewrite Heq.
+      iApply na_own_union. done. iFrame.
+  Qed.
+
+End namespacing.
 
 Section property_ref.
 
 Context `{!heapGS Σ} `{!na_invG Σ}.
 
-Parameter ρ : gname.
+Definition ssref (ℓ : loc) (π : gname) (n : nat) (ϕ : val -> iProp Σ) : iProp Σ :=
+  na_inv π (W n) (∃ v, ϕ v ∗ ℓ ↦ v).
 
-Definition πref (ℓ : loc) (N : namespace) (π : val -> iProp Σ) : iProp Σ :=
-  na_inv ρ N (∃ v, π v ∗ ℓ ↦ v).
+Notation "l ⤇{ π . N } ϕ" := (ssref l π N ϕ) (at level 60).
 
-Notation "l ⤇{ N } π" := (πref l N π) (at level 60).
+Definition Token π n := na_own π (↑ Ξ n).
 
-Global Instance pers_πref ℓ N π : Persistent (πref ℓ N π).
+Global Instance pers_ssref ℓ π N ϕ : Persistent (ssref ℓ π N ϕ).
 Proof. apply _. Qed.
 
-Variable π : val -> iProp Σ.
+Theorem new_pool : ⊢ |==> ∃ π, Token π 0.
+Proof.
+  iStartProof.
+  iMod (na_alloc) as "[%π H]".
+  iModIntro.
+  iExists π.
+  by iDestruct (na_own_acc (↑ Ξ 0) ⊤ with "H") as "[H _]".
+Qed.
 
-Theorem πref_alloc (v : val) : forall N,
-  {{{ π v }}} ref v {{{ ℓ, RET #ℓ; ℓ ⤇{N} π }}}.
+Variable π : gname.
+Variable ϕ : val -> iProp Σ.
+
+Theorem ssref_alloc (v : val) : forall N,
+  {{{ ϕ v }}} ref v {{{ ℓ, RET #ℓ; ℓ ⤇{π . N} ϕ }}}.
 Proof.
   iIntros (N ψ) "Hv Hψ".
   wp_alloc ℓ as "Hℓ".
   iApply "Hψ".
   iFrame "#".
-  iApply (na_inv_alloc ρ _ N (∃ v, π v ∗ ℓ ↦ v) with "[Hv Hℓ]").
+  iApply (na_inv_alloc π _ (W N) (∃ v, ϕ v ∗ ℓ ↦ v) with "[Hv Hℓ]").
     { iNext. iExists v. iFrame. }
 Qed.
 
-(* Unused? TODO confirm or remove this comment *)
-Theorem πref_load `{forall x, Persistent (π x)} (ℓ : loc) : forall N,
-  {{{ ℓ ⤇{N} π ∗ na_own ρ (↑N) }}} ! #ℓ {{{ v', RET v'; π v' ∗ na_own ρ (↑N) }}}.
+(* Unused. *)
+Theorem ssref_load `{forall x, Persistent (ϕ x)} (ℓ : loc) : forall n,
+  {{{ ℓ ⤇{π . n} ϕ ∗ Token π n }}} ! #ℓ {{{ v', RET v'; ϕ v' ∗ Token π n }}}.
 Proof.
-  iIntros (N ψ) "[ι O] Hψ".
+  iIntros (n ψ) "[ι O] Hψ".
+  iDestruct (na_own_acc (↑ W n) with "O") as "[O A]". by apply access_stage.
   iInv "ι" as "[(%v' & #Hv' & Hℓ) O]".
   wp_load.
   iModIntro.
   iSplitL "Hℓ O".
   - iSplitL "Hℓ"; by iFrame "#".
-  - iIntros "H". iApply "Hψ". by iFrame "#".
+  - iIntros "H". iApply "Hψ".
+    iDestruct ("A" with "H") as "H". by iFrame "#".
 Qed.
 
 (* Unused. *)
-Theorem πref_store (ℓ : loc) (x : val) : forall N,
-  {{{ ℓ ⤇{N} π ∗ π x ∗ na_own ρ (↑N) }}} #ℓ <- x {{{ RET #(); na_own ρ (↑N) }}}.
+Theorem ssref_store (ℓ : loc) (x : val) : forall n,
+  {{{ ℓ ⤇{π . n} ϕ ∗ ϕ x ∗ Token π n }}} #ℓ <- x {{{ RET #(); Token π n }}}.
 Proof.
-  iIntros (N ψ) "(#ι & Hx & O) Hψ".
+  iIntros (n ψ) "(#ι & Hx & O) Hψ".
+  iDestruct (na_own_acc (↑ W n) with "O") as "[O A]". by apply access_stage.
   iInv "ι" as "[(%v' & Hv' & Hℓ) O]".
   wp_store.
-  iSplitR "Hψ"; iModIntro.
+  iSplitR "Hψ A"; iModIntro.
   - iSplitR "O"; [| done].
     iExists x. iNext. iFrame.
-  - iIntros "H". by iApply "Hψ".
+  - iIntros "H".
+    iDestruct ("A" with "H") as "O".
+    by iApply "Hψ".
 Qed.
 
-(* TODO eliminate [modify] *)
-Definition modify : val :=
-  λ: "r" "f",
-    let: "v" := !"r" in
-    let: "v'" := "f" "v" in
-    "r" <- "v'";;
-    "v'".
-
-Theorem πref_load_open (ℓ : loc) :
-  ∀ (N N' : namespace), ↑N ⊆@{coPset} ↑N' →
-  {{{ ℓ ⤇{N} π ∗ na_own ρ (↑N') }}} 
-    !#ℓ 
-  {{{ v, RET v; na_own ρ (↑N' ∖ ↑N) ∗ π v ∗
-    ∀ v', ▷ π v' -∗ na_own ρ (↑N' ∖ ↑N) -∗ WP (#ℓ <- v') {{ _, na_own ρ (↑N') }}
+Theorem ssref_load_open (ℓ : loc) : forall n,
+  {{{ ℓ ⤇{π . n} ϕ ∗ Token π n }}}
+    !#ℓ
+  {{{ v, RET v; Token π (S n) ∗ ϕ v ∗
+    ∀ v', ▷ ϕ v' -∗ Token π (S n) -∗ WP (#ℓ <- v') {{ _, Token π n }}
   }}}.
 Proof.
-  iIntros (N N' Hincl ψ) "[#ι O] Hψ".
-  iInv "ι" as "[(%v & Hv & Hℓ) O]" "Hclose".
+  iIntros (n ψ) "[#ι O] Hψ".
+  destruct (own_next_stage π n) as [σ Next].
+  rewrite /Token.
+  rewrite (union_difference_L (↑ W n) (↑ Ξ n)); [| by apply access_stage].
+  iDestruct (na_own_union with "O") as "[OW OX]".
+    { symmetry. by apply namespaces.coPset_disjoint_difference_l1. }
+  iInv "ι" as "[(%v & Hv & Hℓ) O']" "Hclose".
   wp_load.
   iModIntro.
   iApply "Hψ".
   iFrame.
-  iIntros (v') "πv' O".
+  iDestruct (Next with "OX") as "[On Oσ]".
+  iFrame.
+  iIntros (v') "ϕv' O".
   wp_store.
+  iDestruct (Next with "[O Oσ]") as "O". by iFrame.
+  iApply na_own_union.
+    { symmetry.  by apply namespaces.coPset_disjoint_difference_l1. }
+  iFrame.
   iApply "Hclose".
   iFrame.
 Qed.
 
+Theorem ssref_read P `{forall v, Persistent (P v)} (ℓ : loc) : forall n,
+  {{{ ℓ ⤇{π . n} ϕ ∗ Token π n ∗ (∀ v, ϕ v -∗ (P v ∗ ϕ v)) }}} !#ℓ {{{ v', RET v'; P v' ∗ Token π n }}}.
+Proof.
+  iIntros (n ψ) "(Hℓ & O & HP) Hψ".
+  iDestruct (na_own_acc (↑ W n) with "O") as "[O A]". by apply access_stage.
+  iInv "Hℓ" as "[(%v & ϕv & ℓv) O]".
+  wp_load.
+  iModIntro.
+  iDestruct ("HP" with "ϕv") as "[Pv ϕv]".
+  iFrame.
+  iIntros "O".
+  iApply "Hψ".
+  iFrame.
+  by iApply "A".
+Qed.
+
 End property_ref.
 
-Notation "l ⤇ π" := (sref l π) (at level 60).
-Notation "l ⤇{ N } π" := (πref l N π) (at level 60).
+Notation "l ⤇ ϕ" := (csref l ϕ) (at level 60).
+Notation "l ⤇{ π . N } ϕ" := (ssref l π N ϕ) (at level 60).
 
 Section instances.
   Context `{!heapGS Σ} `{!na_invG Σ}.
-  (* TODO  
-  Global Instance isSrefContractive (ℓ : loc) : Contractive (λ π, ℓ ⤇ π).
-  *)
-  Global Instance na_inv_contractive ρ N : Contractive (na_inv ρ N).
+  Global Instance na_inv_contractive π N : Contractive (na_inv π N).
   Proof. solve_contractive. Qed.
 End instances.
