theories/shared_ref_.v
@@ -1,0 +1,164 @@
+
+From iris.base_logic.lib Require Export own na_invariants invariants iprop.
+From iris.heap_lang Require Import lang proofmode notation.
+From iris.algebra Require Import agree.
+
+Section shared_ref.
+
+Context `{!heapGS Σ}.
+
+Let N := nroot .@ "sref".
+
+Definition csref (ℓ : loc) (π : val -> iProp Σ) : iProp Σ :=
+  inv N (∃ v, π v ∗ ℓ ↦ v).
+
+Notation "l ⤇ π" := (csref l π) (at level 60).
+
+Theorem pers_csref : forall ℓ π, Persistent (csref ℓ π).
+Proof. apply _. Qed.
+
+Variable π : val -> iProp Σ.
+
+Theorem csref_alloc (v : val) :
+  {{{ π v }}} ref v {{{ ℓ, RET #ℓ; ℓ ⤇ π }}}.
+Proof.
+  iIntros (ψ) "Hv Hψ".
+  wp_alloc ℓ as "Hℓ".
+  iApply "Hψ".
+  iFrame "#".
+  iApply inv_alloc. iNext.
+  iExists v. by iFrame.
+Qed.
+
+Theorem csref_load `{forall x, Persistent (π x)} (ℓ : loc) :
+  {{{ ℓ ⤇ π }}} ! #ℓ {{{ v', RET v'; π v' }}}.
+Proof.
+  iIntros (ψ) "#ι Hψ".
+  iInv "ι" as "(%v' & #Hv' & Hℓ)".
+  wp_load.
+  iSplitL "Hℓ".
+  - by iFrame "#".
+  - by iApply "Hψ".
+Qed.
+
+Theorem csref_store (ℓ : loc) (x : val) :
+  {{{ ℓ ⤇ π ∗ π x }}} #ℓ <- x {{{ RET #(); True }}}.
+Proof.
+  iIntros (ψ) "(#ι & Hx) Hψ".
+  iInv "ι" as "(%v' & Hv' & Hℓ)".
+  wp_store.
+  iSplitR "Hψ"; [| by iApply "Hψ"].
+  iModIntro. iNext.
+  iExists x. by iFrame.
+Qed.
+
+End shared_ref.
+
+Section alloc.
+  Context `{!heapGS Σ} `{!na_invG Σ}.
+  Theorem na_pool_alloc :
+    ⊢ |==> ∃ p : gname, na_own p ⊤.
+  Proof. by apply na_alloc. Qed.
+End alloc.
+
+Section sequential_stable_ref.
+
+Context `{!heapGS Σ} `{!na_invG Σ}.
+
+(* FIXME(Juliette): leaks from the section somehow *)
+Parameter ρ : gname.
+
+Definition ssref (ℓ : loc) (N : namespace) (π : val -> iProp Σ) : iProp Σ :=
+  na_inv ρ N (∃ v, π v ∗ ℓ ↦ v).
+
+Notation "l ⤇{ N } π" := (ssref l N π) (at level 60).
+
+Global Instance pers_ssref ℓ N π : Persistent (ssref ℓ N π).
+Proof. apply _. Qed.
+
+Variable π : val -> iProp Σ.
+
+Theorem ssref_alloc (v : val) : forall N,
+  {{{ π v }}} ref v {{{ ℓ, RET #ℓ; ℓ ⤇{N} π }}}.
+Proof.
+  iIntros (N ψ) "Hv Hψ".
+  wp_alloc ℓ as "Hℓ".
+  iApply "Hψ".
+  iFrame "#".
+  iApply (na_inv_alloc ρ _ N (∃ v, π v ∗ ℓ ↦ v) with "[Hv Hℓ]").
+    { iNext. iExists v. iFrame. }
+Qed.
+
+(* Unused. *)
+Theorem ssref_load `{forall x, Persistent (π x)} (ℓ : loc) : forall N,
+  {{{ ℓ ⤇{N} π ∗ na_own ρ (↑N) }}} ! #ℓ {{{ v', RET v'; π v' ∗ na_own ρ (↑N) }}}.
+Proof.
+  iIntros (N ψ) "[ι O] Hψ".
+  iInv "ι" as "[(%v' & #Hv' & Hℓ) O]".
+  wp_load.
+  iModIntro.
+  iSplitL "Hℓ O".
+  - iSplitL "Hℓ"; by iFrame "#".
+  - iIntros "H". iApply "Hψ". by iFrame "#".
+Qed.
+
+(* Unused. *)
+Theorem ssref_store (ℓ : loc) (x : val) : forall N,
+  {{{ ℓ ⤇{N} π ∗ π x ∗ na_own ρ (↑N) }}} #ℓ <- x {{{ RET #(); na_own ρ (↑N) }}}.
+Proof.
+  iIntros (N ψ) "(#ι & Hx & O) Hψ".
+  iInv "ι" as "[(%v' & Hv' & Hℓ) O]".
+  wp_store.
+  iSplitR "Hψ"; iModIntro.
+  - iSplitR "O"; [| done].
+    iExists x. iNext. iFrame.
+  - iIntros "H". by iApply "Hψ".
+Qed.
+
+Theorem ssref_load_open (ℓ : loc) :
+  ∀ (N N' : namespace), ↑N ⊆@{coPset} ↑N' →
+  {{{ ℓ ⤇{N} π ∗ na_own ρ (↑N') }}}
+    !#ℓ
+  {{{ v, RET v; na_own ρ (↑N' ∖ ↑N) ∗ π v ∗
+    ∀ v', ▷ π v' -∗ na_own ρ (↑N' ∖ ↑N) -∗ WP (#ℓ <- v') {{ _, na_own ρ (↑N') }}
+  }}}.
+Proof.
+  iIntros (N N' Hincl ψ) "[#ι O] Hψ".
+  iInv "ι" as "[(%v & Hv & Hℓ) O]" "Hclose".
+  wp_load.
+  iModIntro.
+  iApply "Hψ".
+  iFrame.
+  iIntros (v') "πv' O".
+  wp_store.
+  iApply "Hclose".
+  iFrame.
+Qed.
+
+Theorem ssref_read P `{forall v, Persistent (P v)} (ℓ : loc) : forall N,
+  {{{ ℓ ⤇{N} π ∗ na_own ρ (↑N) ∗ (∀ v, π v -∗ (P v ∗ π v)) }}} !#ℓ {{{ v', RET v'; P v' ∗ na_own ρ (↑N) }}}.
+Proof.
+  iIntros (N ψ) "(Hℓ & O & HP) Hψ".
+  iInv "Hℓ" as "[(%v & πv & ℓv) O]".
+  wp_load.
+  iModIntro.
+  iDestruct ("HP" with "πv") as "[Pv πv]".
+  iFrame.
+  iIntros "O".
+  iApply "Hψ".
+  iFrame.
+Qed.
+
+End sequential_stable_ref.
+
+Notation "l ⤇ π" := (csref l π) (at level 60).
+Notation "l ⤇{ N } π" := (ssref l N π) (at level 60).
+
+Section instances.
+  Context `{!heapGS Σ} `{!na_invG Σ}.
+  (* TODO
+  Global Instance isSrefContractive (ℓ : loc) : Contractive (λ π, ℓ ⤇ π).
+  *)
+  Global Instance na_inv_contractive ρ N : Contractive (na_inv ρ N).
+  Proof. solve_contractive. Qed.
+End instances.
